Prove the lifting theorem for unops, binops and ternary ops

Source/DafnyCompilers/CompilerCommon.dfy
@@ -131,7 +131,7 @@ module {:extern "DafnyInDafny.Common"} DafnyCompilerCommon {
         ProperMultiSubset | ProperMultiSuperset | MultisetDisjoint | InMultiset |
         NotInMultiset | MultisetUnion | MultisetIntersection | MultisetDifference |
         MultisetSelect // Separate node in DafnyAST.cs
-      datatype Maps =
+      datatype Maps = // TODO: MapSubtraction -> MapSubstraction? (with an "s"?)
         MapEq | MapNeq | InMap | NotInMap | MapMerge | MapSubtraction |
         MapSelect // Separate node in DafnyAST.cs
       datatype Datatypes =
